Chapter 8

ch8.v
@@ -1,5 +1,6 @@
 Require Import List.
 Require Import JMeq.
+Require Import ZArith.
 Import ListNotations.
 
 (* Exercise 8.1 *)
@@ -266,7 +267,7 @@ Fixpoint bin_to_string' (t:bin) : list par :=
     app (bin_to_string' u) (cons open (app (bin_to_string' v) (cons close nil)))
   end.
 
-Theorem bin_to_string_wp' : forall b, wp (bin_to_string' b).
+Theorem bin_to_string'_wp : forall b, wp (bin_to_string' b).
 Proof.
   intros.
   induction b; simpl.
@@ -284,3 +285,858 @@ Proof.
   - intros; rewrite IHx. auto.
 Qed.
 
+(* Exercise 8.9 *)
+(* Prove that an even number is the double of another number. *)
+
+Inductive even : nat -> Prop :=
+  | O_even : even O
+  | p2_even : forall n, even n -> even (S (S n)).
+
+Goal forall n, even n -> exists x, 2*x = n.
+Proof.
+  intros.
+  induction H.
+  - exists 0; auto.
+  - destruct IHeven as [x Hdouble].
+    exists (1 + x).
+    rewrite PeanoNat.Nat.mul_add_distr_l.
+    rewrite Hdouble; auto.
+Qed.
+    
+(* Exercise 8.10 *)
+(* Prove that the double of a number is always even. This proof requires an induction
+  with the usual induction principle. Then show that the square of an even number is
+  always even, this time with an induction on the even predicate.*)
+
+Theorem double_even : forall n, even (n+n).
+Proof.
+  induction n; simpl.
+  - constructor.
+  - rewrite PeanoNat.Nat.add_succ_r.
+    apply p2_even, IHn.
+Qed.
+
+Lemma add_even : forall n m, even n -> even m -> even (n + m).
+Proof.
+  intros n m H.
+  induction H; simpl; intros.
+  - auto.
+  - apply p2_even, IHeven; auto.
+Qed.
+
+Goal forall n, even n -> even (n*n).
+Proof.
+  intros.
+  induction H; simpl.
+  - constructor.
+  - apply p2_even.
+    rewrite 2 PeanoNat.Nat.add_succ_r.
+    apply p2_even.
+    rewrite PeanoNat.Nat.add_assoc.
+    apply add_even.
+    + apply double_even.
+    + repeat rewrite PeanoNat.Nat.mul_succ_r.
+      rewrite <- PeanoNat.Nat.add_assoc.
+      apply add_even; auto.
+      apply double_even.
+Qed.
+
+(* Exercise 8.11 *)
+(* Redo the following proof, using the tactic apply instead of elim: *)
+
+Theorem lt_le: forall n p: nat, n < p -> n <= p.
+Proof.
+  intros n p H; elim H; repeat constructor; assumption.
+Qed.
+
+Goal forall n p: nat, n < p -> n <= p.
+Proof.
+  intros n p H; apply le_S_n; constructor; assumption.
+Qed.
+
+(* Exercise 8.12 *)
+(* Prove by induction on le that the inductive definition 
+  implies the impredicative version given in Sect. 5.5.4.1: *)
+Definition my_le (n p : nat) :=
+  forall P : nat -> Prop, P n -> (forall q, P q -> P (S q)) -> P p.
+
+Theorem le_my_le: forall n p: nat, n <= p -> my_le n p.
+Proof.
+  intros n p H.
+  induction H; intros P HP HS.
+  - assumption.
+  - apply HS, IHle.
+    + apply HP.
+    + apply HS.
+Qed.
+
+(* Exercise 8.13 *)
+(* Use induction to prove that le is transitive
+  (this proof is already in the Coq libraries, do not use it). *)
+
+Theorem le_trans': forall n p q: nat, n < p -> p < q -> n < q.
+Proof.
+  intros n p q H.
+  induction H; intros.
+  - apply PeanoNat.Nat.lt_succ_l; auto.
+  - apply IHle, PeanoNat.Nat.lt_succ_l; auto.
+Qed.
+
+(* Compare this proof with the proof of transitivity for my_le
+  (without using the equivalence between le and my_le). *)
+
+Theorem my_le_trans: forall n p q: nat, my_le n p -> my_le p q -> my_le n q.
+Proof.
+  intros n p q Hnp Hpq P HP H.
+  apply Hpq.
+  - apply Hnp.
+    + apply HP.
+    + apply H.
+  - apply H.
+Qed. 
+
+(* Exercise 8.14 (proposed by J.F. Monin) *)
+(* Here is another definition of <:
+    n < m iff exists x:nat, x+n = m
+  This can be written as an inductive definition in the following manner: *)
+
+  Inductive le_diff (n m : nat) : Prop := 
+    le_d: forall x: nat, x+n = m -> le_diff n m.
+
+(* The variable x can be interpreted as the height of a proof tree for n <= m. 
+  Prove the equivalence between le and le_diff. *)
+
+Theorem le_le_diff_equiv: forall n m, n <= m <-> le_diff n m.
+Proof.
+  split; intros.
+  - induction H.
+    + apply (le_d _ _ 0). auto.
+    + inversion IHle as [x Hx].
+      apply (le_d _ _ (S x)).
+      simpl; auto.
+  - destruct H; subst.
+    induction x; simpl.
+    + constructor.
+    + constructor; assumption.
+Qed.
+
+(* Exercise 8.15 *)
+(* An alternative description of the order < on nat is the following one: *)
+
+  Inductive le': nat -> nat -> Prop :=
+  | le'_O_p : forall p: nat, le' 0 p
+  | le'_Sn_Sp : forall n p: nat, le' n p -> le' (S n) (S p).
+
+(* Prove that le and le' are equivalent. *)
+
+Theorem le_le'_equiv: forall n m, n <= m <-> le' n m.
+Proof.
+  split.
+  - revert m; induction n; intros.
+    + constructor.
+    + destruct m.
+      * inversion H.
+      * constructor.
+        apply IHn, le_S_n.
+        assumption.
+  - intros H; induction H.
+    + induction p.
+      * constructor.
+      * constructor; assumption.
+    + apply le_n_S.
+      assumption.
+Qed.
+
+(* Exercise 8.16 *)
+(* An alternative description of sorted lists is the following one: *)
+  Definition sorted' (A: Set) (R: A->A->Prop) (l: list A) := 
+    forall (l1 l2: list A) (n1 n2: A),
+      l = app l1 (cons n1 (cons n2 l2)) -> R n1 n2. 
+(* Prove that sorted and sorted' are equivalent. *)
+
+Inductive sorted (A: Set) (R: A->A->Prop): list A -> Prop :=
+  | sorted0: sorted A R nil
+  | sorted1: forall x:A, sorted A R (cons x nil)
+  | sorted2: forall (x y:A) (l:list A), R x y -> sorted A R (cons y l) -> sorted A R (cons x (cons y l)).
+
+
+Lemma trim_sorted': forall A R a l, sorted' A R (a :: l) -> sorted' A R l.
+Proof.
+  intros A R a l.
+  induction l; intros;
+  unfold sorted'; intros l1 l2 n1 n2 Heq.
+  - destruct l1; inversion Heq.
+  - apply (H (a :: l1) l2); simpl.
+    rewrite Heq. auto.
+Qed.
+
+Theorem sorted_sorted'_equiv: forall A R l, sorted A R l <-> sorted' A R l.
+Proof.
+  split; intros.
+  - induction H; intros l1 l2 n1 n2 ?H.
+    + destruct l1; inversion H.
+    + destruct l1; inversion H.
+      destruct l1; inversion H2.
+    + unfold sorted' in IHsorted.
+      destruct l1; simpl in H1.
+      * inversion H1; subst. assumption.
+      * inversion H1.
+        apply (IHsorted l1 l2). assumption.
+  - induction l; [constructor|].
+    destruct l; constructor.
+    + apply (H [] l); auto.
+    + apply trim_sorted' in H; auto.
+Qed.
+
+(* Exercise 8.17 *)
+(* What is the systematic way to translate an inductive definition
+  into an impredicative definition? Propose a method and test it on the
+  examples given in Sect. 5.5. For each case, prove the equivalence
+  between the inductive definition and the impredicative dernition. *)
+
+(* From the inductive defintion, take the generated induction principle.
+  Remove all instances of the inductive predicate from implications in
+  the inductive principle, and instead imply the consequent directly. 
+  Also, strictly for readability, move all dependant products except
+  the last (forall P: Prop) into the header as arguments. This will
+  match its header signature with the inductive definition.
+*)
+
+Check True_ind. (* forall P : Prop, P -> True -> P *)
+Check False_ind. (* forall P : Prop, False -> P *)
+Check and_ind. (* forall A B P : Prop, (A -> B -> P) -> A /\ B -> P *)
+Check or_ind. (* forall A B P : Prop, (A -> P) -> (B -> P) -> A \/ B -> P *)
+Check ex_ind. (* forall (A : Type) (P : A -> Prop) (P0 : Prop), (forall x : A, P x -> P0) -> (exists y, P y) -> P0 *)
+Check le_ind. (* forall (n : nat) (P : nat -> Prop), P n -> (forall m : nat, n <= m -> P m -> P (S m)) -> forall n0 : nat, n <= n0 -> P n0 *)
+
+Definition my_True := forall P: Prop, P -> P.
+Definition my_False := forall P: Prop, P.
+Definition my_and (P Q:Prop) := forall R: Prop, (P->Q->R) -> R.
+Definition my_or (P Q:Prop) := forall R: Prop, (P->R)->(Q->R) -> R.
+Definition my_ex (A:Set) (P:A->Prop) := forall R: Prop, (forall x:A, P x -> R) -> R.
+(* Definition my_le (n p : nat) :=
+  forall P : nat -> Prop, P n -> (forall q, P q -> P (S q)) -> P p. *)
+
+Goal True <-> my_True.
+Proof. split; auto. intros T P; auto. Qed.
+
+Goal False <-> my_False.
+Proof. split; intros H; [elim H | apply H]. Qed.
+
+Goal forall P Q, and P Q <-> my_and P Q.
+Proof.
+  split; intros.
+  - unfold my_and; elim H; auto.
+  - split; apply H; intros; auto.
+Qed.
+
+Goal forall P Q, or P Q <-> my_or P Q.
+Proof.
+  split; intros.
+  - unfold my_or; elim H; auto.
+  - apply H; auto.
+Qed.
+
+Goal forall A P, ex P <-> my_ex A P.
+Proof.
+  split; intros.
+  - unfold my_ex; elim H; intros x HP R Hex.
+    apply (Hex x), HP.
+  - apply H; intros x HP.
+    exists x; auto.
+Qed.
+
+Goal forall n m, le n m <-> my_le n m.
+Proof.
+  split; [apply le_my_le|].
+  unfold my_le; intros.
+  apply H.
+  - constructor.
+  - intros q Hle.
+    constructor; auto.
+Qed.
+
+(* Exercise 8.18 (proposed by H. Südbrock) *)
+(* Carry on with the following development: *)
+(* We advise the reader to prove a few lemmas before attacking
+  the main theorem. Actually, this exercise is interesting mainly for 
+  the choice of lemmas. *)
+
+Section weird_induc_proof.
+  Variable P : nat->Prop. 
+  Variable f : nat->nat.
+
+  Hypothesis f_strict_mono: forall n p:nat, 
+    lt n p -> lt (f n) (f p).
+  Hypothesis f_0 : lt 0 (f 0).
+
+  Hypothesis PO: P 0.
+  Hypothesis P_Sn_n: forall n:nat, P (S n) -> P n.
+  Hypothesis f_P: forall n:nat, P n -> P (f n).
+
+  (* Using P_Sn_n we can show (P n) also covers all cases less than n *)
+  Lemma P_le: forall n m, n <= m -> P m -> P n.
+  Proof. intros n m Hle HP. induction Hle; auto. Qed.
+
+  (* Then using f_P we can show that for any n, there exists a number 
+    greater than or equal to n that is the result of repeated
+    applications of f on 0, and that that number is also covered *)
+  Fixpoint iter (i n:nat) : nat :=
+  match i with
+  | O => n
+  | S i' => f (iter i' n)
+  end.
+
+  Lemma iter_incr : forall i, iter i 0 < iter (S i) 0.
+  Proof. induction i; simpl; auto. Qed.
+  
+  Lemma i_iter_lt: forall i:nat, i <= iter i 0.
+  Proof.
+    induction i; auto.
+    pose proof (iter_incr i).
+    eapply PeanoNat.Nat.le_lt_trans.
+    - apply IHi.
+    - auto.
+  Qed.
+
+  Lemma P_iter: forall i, P (iter i 0).
+  Proof. induction i; simpl; auto. Qed.
+
+  (* Therefore given any n, there exists a number m s.t. n <= m \/ P m 
+    and since P m -> for all n <= m, P n, we have a proof for any P n *)
+  Theorem weird_induc: forall n:nat, P n.
+  Proof.
+    intros. 
+    eapply P_le.
+    - apply i_iter_lt.
+    - apply P_iter.
+  Qed.
+
+End weird_induc_proof.
+
+(* Exercise 8.19 *)
+(* This exercise continues Exercise 8.5, page 216. Here is a
+  second definition of well-parenthesized expressions. Prove that
+  it is equivalent to the previous one: *)
+Inductive wp': list par -> Prop :=
+| wp'_nil: wp' nil
+| wp'_cons: forall l1 l2: list par, wp' l1 -> wp' l2 ->
+    wp' (cons open (app l1 (cons close l2))).
+
+Theorem wp'_wp: forall l, wp' l -> wp l.
+Proof.
+  intros l H; induction H.
+  - constructor.
+  - change (wp ([open] ++ l1 ++ [close] ++ l2)).
+    rewrite 2 app_assoc.
+    apply wp_concat; simpl.
+    + constructor; auto.
+    + auto.
+Qed.
+
+Theorem wp_wp': forall l, wp l -> wp' l.
+Proof.
+  intros; induction H.
+  - constructor.
+  - constructor; [auto|constructor].
+  - induction IHwp1; simpl; auto.
+    rewrite <- app_assoc; simpl.
+    constructor; auto.
+    apply IHIHwp1_2, wp'_wp; auto.
+Qed.
+
+Theorem wp_wp'_equiv: forall l, wp l <-> wp' l.
+Proof.
+  split.
+  - apply wp_wp'.
+  - apply wp'_wp.
+Qed.
+
+(* Exercise 8.20 *)
+(* This exercise continues Exercise 8.19. Here is a
+  third deftnition. Prove that it is equivalent to the previous ones: *)
+Inductive wp'': list par -> Prop :=
+  | wp''_nil: wp'' nil
+  | wp''_cons: forall l1 l2: list par, wp'' l1 -> wp'' l2
+    -> wp'' (app l1 (cons open (app l2 (cons close nil)))).
+  
+Theorem wp''_wp: forall l, wp'' l -> wp l.
+Proof.
+  intros l H; induction H.
+  - constructor.
+  - apply wp_concat.
+    + auto.
+    + constructor; auto.
+Qed.
+
+Theorem wp_wp'': forall l, wp l -> wp'' l.
+Proof.
+  intros; induction H.
+  - constructor.
+  - apply (wp''_cons nil); [constructor|auto].
+  - induction IHwp2; simpl.
+    + rewrite app_nil_r; auto.
+    + rewrite app_assoc; simpl.
+      constructor; auto.
+      apply IHIHwp2_1, wp''_wp; auto.
+Qed.
+
+Theorem wp_wp''_equiv: forall l, wp l <-> wp'' l.
+Proof.
+  split.
+  - apply wp_wp''.
+  - apply wp''_wp.
+Qed.
+
+(* Exercise 8.21 *)
+(* This exercise continues Exercise 8.20. Here is a function that
+ recognizes well-parenthesized expressions by counting the opening
+ parentheses that are not yet closed: *)
+
+  Fixpoint recognize (n:nat) (l:list par): bool :=
+    match l with
+    | nil => match n with 0 => true | _ => false end
+    | cons open l' => recognize (S n) l'
+    | cons close l' =>
+      match n with 0 => false | S n' => recognize n' l' end 
+    end.
+
+(* Prove the following theorem: *)
+
+Theorem recognize_complete_aux: forall l: list par,
+  wp l -> forall (n:nat) (l':list par),
+    recognize n (app l l' ) = recognize n l'.
+Proof.
+  intros l H.
+  rewrite wp_wp'_equiv in H.
+  induction H; intros; simpl; auto.
+  rewrite <- app_assoc; simpl.
+  rewrite IHwp'1; simpl.
+  apply IHwp'2.
+Qed.
+
+(* Conclude with the following main theorem: *)
+
+Theorem recognize_complete: forall l:list par,
+  wp l -> recognize 0 l = true.
+Proof.
+  intros l H.
+  induction H; simpl; [auto| |];
+  rewrite recognize_complete_aux; auto.
+Qed.
+
+(* Exercise 8.22 *)
+(* This exercise is rather hard and continues Exercise 8.21.
+  Prove that the recognize function only accepts well-parenthesized
+  expressions, More precisely: *)
+
+Fixpoint opens (n : nat): list par :=
+  match n with
+  | O => nil
+  | S n' => open :: opens n'
+  end.
+
+Lemma opens_app: forall n, opens (S n) = opens n ++ [open].
+Proof.
+  induction n; simpl; [|rewrite <- IHn]; auto.
+Qed.
+
+Lemma wp_pair: wp [open; close].
+Proof.
+  change (wp (open :: nil ++ [close])).
+  apply wp_nest. apply wp_nil.
+Qed.
+
+Theorem app_decompose :
+ forall (A:Type) (l1 l2 l3 l4:list A),
+   l1 ++ l2 = l3 ++ l4 ->
+   (exists l1' : list A, l1 = l3 ++ l1' /\ l4 = l1' ++ l2) \/
+   (exists a : A,
+      exists l2' : list A, l3 = l1 ++ a :: l2' /\ l2 = (a :: l2') ++ l4).
+Proof.
+  simple induction l1.
+  - intros l2 l3; case l3.
+    + intros l4 H; left; exists (nil (A:=A)); auto.
+    + intros a l3' Heq; right; exists a; exists l3'; auto.
+  - clear l1; intros a l1 Hrec l2 l3; case l3.
+    + intros l4 H; left; exists (a :: l1); auto.
+    + simpl ; intros a' l3' l4 Heq; injection Heq; intros Heq' Heq''.
+      elim Hrec with (1 := Heq').
+      intros [l1' [Heq3 Heq4]]; left; exists l1'; split; auto.
+      rewrite Heq''; rewrite Heq3; auto.
+      intros [a'' [l2' [Heq3 Heq4]]]; right; exists a'', l2'; split; auto.
+      rewrite Heq''; rewrite Heq3; auto.
+Qed.
+
+Local Hint Resolve wp_pair : core.
+Theorem wp_remove_oc_aux :
+forall l:list par,
+  wp l ->
+  forall l1 l2:list par, l1 ++ l2 = l -> wp (l1 ++ open :: close :: l2).
+Proof.
+  intros l H; elim H.
+  - intros l1 l2 Heq.
+    destruct (app_eq_nil _ _ Heq).
+    subst; auto.
+  - clear l H; intros l Hl IHl l1 l2 Heq.
+    rewrite app_comm_cons in Heq.
+    elim (app_decompose _ _ _ _ _ Heq).
+    + intros [l1' [Heq1 Heq2]].
+      destruct l1'; simpl in *; subst.
+      * simpl; rewrite app_nil_r.
+        change (wp (open :: l ++ [open; close] ++ [close])).
+        rewrite app_assoc.
+        apply wp_nest, wp_concat; auto.
+      * inversion Heq2.
+        symmetry in H1; destruct (app_eq_nil _ _ H1).
+        subst. apply wp_concat; [apply wp_nest|]; auto.
+    + intros [a [l2' [Heq1 Heq2]]].
+      destruct l1; simpl in *.
+      * change (wp ([open;close] ++ l2)).
+        apply wp_concat; auto.
+        subst; apply wp_nest; auto.
+      * subst; inversion Heq1.
+        change (wp ([open] ++ l1 ++ open :: close :: a :: l2' ++ [close])).
+        repeat rewrite app_comm_cons.
+        rewrite (app_assoc l1).
+        apply wp_nest, IHl; auto.
+  - intros l1 l2 Hp1 Hr1 Hp2 Hr2 l3 l4 Heq.
+    elim (app_decompose _ _ _ _ _ Heq).
+    intros [l1' [Heq1 Heq2]]; rewrite Heq1, <- app_assoc;
+    apply wp_concat; auto.
+    intros [a' [l2' [Heq1 Heq2]]].
+    rewrite Heq2, !app_comm_cons, app_assoc.
+    apply wp_concat; auto.
+Qed.
+
+Lemma recognize_sound_aux: forall n l,
+  recognize n l = true -> wp ((opens n) ++ l).
+Proof.
+  intros n l; revert n.
+  induction l; simpl; intros.
+  - destruct n; [|discriminate].
+    simpl; constructor.
+  - destruct a.
+    + change (wp (opens n ++ [open] ++ l)).
+      rewrite app_assoc, <- opens_app. auto.
+    + destruct n; [discriminate|].
+      rewrite opens_app, <- app_assoc.
+      change (wp (opens n ++ open :: close :: l)).
+      apply (wp_remove_oc_aux (opens n ++ l)); auto.
+Qed.
+
+Theorem recognize_sound: forall l: list par, recognize 0 l = true -> wp l.
+Proof.
+  intros l H; apply (recognize_sound_aux _ _ H).
+Qed.
+
+(* Exercise 8.23 *)
+(* This exercise continues Exercises 8.7 and 8.20. 
+  We consider the following parsing function: *)
+
+Fixpoint parse (s:list bin) (t:bin) (l:list par): option bin :=
+  match l with
+  | nil => match s with nil => Some t | _ => None end
+  | cons open l' => parse (cons t s) L l'
+  | cons close l' =>
+    match s with
+    | cons t' s' => parse s' (N t' t) l'
+    | _ => None
+    end
+  end.
+
+(* Prove that this parser is correct and complete: *)
+
+Theorem parse_reject_indep_t :
+  forall (l:list par) (s:list bin) (t:bin),
+    parse s t l = None ->
+    forall (s':list bin) (t':bin),
+      length s' = length s -> parse s' t' l = None.
+Proof.
+  induction l; simpl;
+  intros s t Heq s' t' Hlen.
+  - destruct s; simpl in *.
+    + inversion Heq.
+    + destruct s'.
+      * discriminate.
+      * auto.
+  - destruct a; simpl.
+    + apply (IHl _ _ Heq); simpl; auto.
+    + destruct s; destruct s';
+      simpl in *; auto.
+      * discriminate.
+      * apply (IHl _ _ Heq); auto.
+Qed.
+
+Theorem parse_complete_aux: forall l: list par,
+  wp' l -> 
+  forall s t l', 
+    parse s t (l ++ l') = None ->
+    forall s' t',
+      length s' = length s -> parse s' t' l' = None.
+Proof.
+  simple induction 1; simpl.
+  - intros; eapply parse_reject_indep_t; eauto.
+  - intros l1 l2 Hl1 IHl1 Hl2 IHl2 s t l' Heq s' t' Hlen.
+    change (close :: l2) with ([close] ++ l2) in Heq.
+    rewrite <- app_assoc in Heq.
+    eapply IHl1 with (s':=t::s) (t':= L) in Heq; auto.
+    rewrite <- app_assoc in Heq; simpl in Heq.
+    eapply IHl2; eauto.
+Qed.
+
+Theorem parse_complete: forall l: list par,
+  wp l -> parse nil L l <> None.
+Proof.
+  intros l H.
+  replace l with (l ++ nil) by apply app_nil_r.
+  intro HF.
+  eapply parse_complete_aux with (s':= nil) (t':=L) in HF.
+  - simpl in HF. discriminate.
+  - apply wp_wp'; auto.
+  - auto.
+Qed.
+
+Fixpoint unparse_stack (s:list bin): list par :=
+  match s with
+  | nil => nil
+  | t :: s' => unparse_stack s' ++ bin_to_string' t ++ [open]
+  end.
+ 
+Theorem parse_invert_aux: forall (l:list par) (s:list bin) (t t':bin),
+  parse s t l = Some t' ->
+  bin_to_string' t' = unparse_stack s ++ bin_to_string' t ++ l.
+Proof.
+  induction l; simpl; intros.
+  - rewrite app_nil_r.
+    destruct s; simpl.
+    + inversion H; subst; auto.
+    + discriminate.
+  - destruct a.
+    + apply IHl in H; simpl in H.
+      repeat rewrite <- app_assoc in H.
+      auto.
+    + destruct s; [discriminate|]; simpl.
+      apply IHl in H; rewrite H; simpl.
+      repeat (rewrite <- app_assoc; simpl).
+      repeat apply f_equal; auto.
+Qed.
+
+Theorem parse_invert: forall (l:list par) (t:bin),
+  parse nil L l = Some t -> bin_to_string' t = l.
+Proof.
+  intros l t H; apply parse_invert_aux in H; simpl in H; auto.
+Qed.
+
+Theorem parse_sound: forall (l:list par) (t:bin),
+  parse nil L l = Some t -> wp l.
+Proof.
+  intros l t H; apply parse_invert in H.
+  subst. apply bin_to_string'_wp.
+Qed.
+
+(* Exercise 8.24 *)
+(* This exercise continues Exercise 8.7 page 217. The following
+  inductive definition gives the description of a parsing function for 
+  well parenthesized expressions. Intuitively, "parse_rel l1 l2 t" reads
+  as "parsing the string l1 leaves l2 as suffix and builds the tree t". *)
+
+Inductive parse_rel: list par -> list par -> bin -> Prop :=
+  | parse_node: 
+    forall (l1 l2 l3:list par) (t1 t2:bin),
+      parse_rel l1 (cons close l2) t1 -> parse_rel l2 l3 t2 -> 
+      parse_rel (cons open l1) l3 (N t1 t2)
+  | parse_leaf_nil: parse_rel nil nil L
+  | parse_leaf_close:
+    forall l : list par, parse_rel (cons close l) (cons close l) L.
+
+(* Prove the following lemmas: *)
+
+Lemma parse_rel_sound_aux: forall (l l': list par) (t:bin),
+  parse_rel l l' t -> l = app (bin_to_string t) l'.
+Proof.
+  simple induction 1; simpl; auto.
+  intros l1 l2 l3 t1 t2 Hl1 Heq1 Hl2 Heq2.
+  subst l1; rewrite <- app_assoc, <- app_comm_cons.
+  repeat apply f_equal; auto.
+Qed.
+
+Lemma parse_rel_sound:
+  forall l:list par, (exists t:bin, parse_rel l nil t) -> wp l.
+Proof.
+  intros l [t H].
+  assert (l = bin_to_string t) as Heq.
+  - rewrite <- app_nil_r. apply parse_rel_sound_aux. auto.
+  - subst. apply bin_to_string_wp.
+Qed.
+
+Section little_semantics.
+
+Variables Var aExp bExp : Set.
+Inductive inst : Set :=
+  | Skip : inst
+  | Assign : Var->aExp->inst
+  | Sequence : inst->inst->inst
+  | WhileDo : bExp->inst->inst.
+
+Variables
+  (state : Set)
+  (update: state->Var->Z -> option state)
+  (evalA: state->aExp -> option Z)
+  (evalB: state->bExp -> option bool).
+
+Inductive exec: state->inst->state->Prop :=
+  | execSkip: forall s:state, exec s Skip s
+  | execAssign: forall (s s1:state) (v: Var) (n:Z) (a: aExp),
+      evalA s a = Some n -> update s v n = Some s1 ->
+      exec s (Assign v a) s1
+  | execSequence: forall (s s1 s2:state) (i1 i2:inst),
+      exec s i1 s1 -> exec s1 i2 s2 ->
+      exec s (Sequence i1 i2) s2
+  | execWhileFalse: forall (s:state) (i:inst) (e:bExp),
+      evalB s e = Some false -> exec s (WhileDo e i) s
+  | execWhileTrue: forall (s s1 s2:state) (i:inst) (e:bExp),
+      evalB s e = Some true -> exec s i s1 ->
+      exec s1 (WhileDo e i) s2 ->
+      exec s (WhileDo e i) s2.
+
+Theorem HoareWhileRule: 
+  forall (P:state->Prop) (b:bExp) (i: inst) (s s':state),
+    (forall s1 s2:state, 
+      P s1 -> evalB s1 b = Some true -> exec s1 i s2 -> P s2) ->
+      P s -> exec s (WhileDo b i) s' ->
+      P s' /\ evalB s' b = Some false.
+Proof.
+  intros P b i s s' H Hp Hexec.
+  remember (WhileDo b i) as i'.
+  induction Hexec; intros;
+  inversion Heqi'; subst; auto.
+  apply IHHexec2; auto.
+  apply (H s s1); auto.
+Qed.
+
+(* Exercise 8.25 *)
+(* Find a method that avoids using an equality, just by
+  making "WhileDo b i" occur in the goal. Prove the theorem
+  again using this method. *)
+
+Definition whileProjB (d:bExp) (i:inst): bExp :=
+  match i with
+  | WhileDo b _ => b
+  | _ => d
+  end.
+
+Definition whileProjI (i: inst): inst :=
+  match i with
+  | WhileDo _ i' => i'
+  | _ => i
+  end.
+
+Definition isWhile (i: inst): Prop :=
+  match i with
+  | WhileDo _ _ => True
+  | _ => False
+  end.
+
+Theorem HoareWhileRule_aux: 
+  forall (P:state->Prop) (b:bExp) (i: inst) (s s':state),
+    (forall s1 s2:state, 
+      P s1 -> evalB s1 (whileProjB b (WhileDo b i)) = Some true ->
+      exec s1 (whileProjI (WhileDo b i) ) s2 -> P s2) ->
+      P s -> exec s (WhileDo b i) s' ->
+      P s' /\ evalB s' (whileProjB b (WhileDo b i)) = Some false.
+Proof.
+  intros P b i s s' Hinvar HP Hexec.
+  generalize (I: isWhile (WhileDo b i)).
+  revert HP Hinvar; elim Hexec; 
+  try contradiction; auto.
+  simpl in *.
+  intros s1 s2 s3 i' e Heval Hexec1 IH1 Hexec2 IH2 HP IHinvar _.
+  apply IH2; auto.
+  apply (IHinvar s1); auto.
+Qed.
+
+Theorem HoareWhileRule':
+  forall (P:state->Prop) (b:bExp) (i: inst) (s s':state),
+    (forall s1 s2:state, 
+      P s1 -> evalB s1 b = Some true -> exec s1 i s2 -> P s2) ->
+      P s -> exec s (WhileDo b i) s' ->
+      P s' /\ evalB s' b = Some false.
+Proof.
+  intros; eapply HoareWhileRule_aux; eauto.
+Qed.
+
+(* Exercise 8.26 *)
+(* Prove that if b evaluates to true in the state s and the
+  loop body is the Skip instruction, then execution never terminates.
+  Here is the statement: *)
+
+Lemma skip_loop_aux: forall (s s': state) (i:inst),
+  exec s i s' ->
+  forall b, i = WhileDo b Skip -> evalB s b = Some true -> False.
+Proof.
+  intros s s' i H.
+  elim H; try discriminate.
+  - intros s1 i' bf Heval1 bt Heq Heval2.
+    inversion Heq; subst.
+    rewrite Heval1 in Heval2.
+    discriminate.
+  - intros s0 s1 s2 i0 bt Heval1 Hexec1 IH1 Hexec2 IH2 bt' Heq Heval2.
+    inversion Heq; subst.
+    inversion Hexec1; subst.
+    eapply IH2; eauto.
+Qed.
+
+Theorem skip_loop: forall (s s':state) (b:bExp),
+  exec s (WhileDo b Skip) s' -> evalB s b = Some true -> False.
+Proof.
+  intros s s' b H Heval.
+  eapply skip_loop_aux; eauto.
+Qed.
+
+(* Exercise 8.27 *)
+(* Prove the Hoare logic rule for sequences. *)
+Theorem HoareSequenceRule :
+ forall (P1 P2 P3:state->Prop)(i1 i2:inst)(s s':state),
+  (forall s1 s2, exec s1 i1 s2 -> P1 s1 -> P2 s2)->
+  (forall s1 s2, exec s1 i2 s2 -> P2 s1 -> P3 s2)->
+  exec s (Sequence i1 i2) s' -> P1 s -> P3 s'.
+Proof.
+  intros P1 P2 P3 i1 i2 s s' H1 H2 Hexec HP1.
+  inversion Hexec; subst.
+  eapply H2; eauto.
+Qed.
+
+End little_semantics.
+
+(* Exercise 8.28 *)
+(* Prove that the list 1;3;2 is not sorted (the definition
+  of sorted is given in Sect. 8.1.1): *)
+
+Goal ~sorted nat le (1::3::2::nil).
+Proof.
+  intro.
+  inversion H; subst.
+  inversion H4; subst.
+  inversion H3.
+  inversion H1.
+  inversion H7.
+Qed.
+
+(* Exercise 8.29 (Proposed by L. Théry) *)
+(* Prove that using stamps of 5 cents and stamps of 3 cents, one can pay all amounts greater than 
+  or equal to 8 cents. This is the Frobenius problem, instantiated for 3 and 5. *)
+
+Import Lia.
+
+Theorem frobenius: forall n, 8 <= n -> exists p q, n = 3*p + 5*q.
+Proof.
+  intros.
+  induction H as [| m Hm IHm].
+  - exists 1, 1; auto.
+  - destruct IHm as [a [b Heq]].
+    assert (3 <= a \/ 1 <= b) as [Ha | Hb].
+    { destruct b; try lia. }
+    + exists (a - 3), (b + 2); lia.
+    + exists (a + 2), (b - 1); lia.
+Qed.
